# 1.3 Exercises

## Concepts

1. $6x$, $6x(3x^2+5)$
2. .
3. $12$, $8$, $6$, $2$, $(x+6)(x+2)$
4. .
5. $A^2 - B^2$, $36 - x^2$
6. .
7. $A + B$, $x + 5$
8. .

## Skills

9. Binomial, $5x^3$ and $6$, $3$
10. .
11. Monomial, $-8$, $0$
12. .
13. Quadronomial? $x$, $-x^2$, $x^3$, $-x^4$, $4$
14. .
15. $7x+5$
16. .
17. $x^2+2x-3$
18. .
19. $5x^3+3x^2+4x-2$
20. .
21. $16x+40-7x+63$ = $9x+103$
22. .
23. $x^5+3x^4-2x^5+6x^3$ = $-x^5+3x^4+6x^3$
24. .
25. $4x^2-8x-2x^2+8x+2x^3-2x^2$ = $2x^3$
26. .
27. $21t^2-12t-14t+8$ = $21t^2-26t+8$
28. .
29. $6x^2-3x+10x-5$ = $6x^2+7x-5$
30. .
31. $2x^2-xy+6xy-3y^2$ = $2x^2+5xy-3y^2$
32. .
33. $16x^2+24x+9$
34. .
35. $y^2-6xy+9x^2$
36. .
37. $4x^2+12xy+9y^2$
38. .
39. $w^2-49$
40. .
41. $9x^2-16$
42. .
43. $x-4$
44. .
45. $a^3+3a^2b+3ab^2+b^3$ --> $y^3+3(y)^2(2)+3(y)(2)^2+8$ = $y^3+6y^2+12y+8$
46. .
47. $x(x^2+2x+3)+2(x^2+2x+3)$ = $x^3+2x^2+3x+2x^2+4x+6$ = $x^3+4x^2+7x+6$
48. .
49. $2x(x^2-x+1)-5(x^2-x+1)$ = $2x^3-2x^2+2x-5x^2+5x-5$ = $2x^3-7x^2+7x-5$
50. .
51. $x\sqrt{ x }-x$
52. .
53. $y^2+y$
54. .
55. $x-y$
56. .
57. $x^4-a^4$
58. .
59. $a-b^2$
60. .
61. $(x-1)^2-x^4$ = $-x^4+x^2-2x+1$
62. .
63. $[(2x+y)-3][(2x+y)+3]$ = $(2x+y)^2-9$ = $4x^2+4xy+y^2-9$
64. .
65. $x^2(4x^2-1)$ or $(2x^2-x)(2x^2+x)$ or $x^2(2x-1)(2x+1)$
66. .
67. $(y-6)(y+9)$
68. .
69. $2xy^2(2x^2-3y+4xy^2)$
70. .
71. $(x+3)^4(x+2)^2[(x+3)-(x+2)]$ = $(x+3)^4(x+2)^2$
72. .
73. $(z-9)(z-2)$
74. .
75. $(5x-2)(2x-3)$
76. .
77. $(3x-1)(x-5)$
78. .
79. $[(3x+2)+6][(3x+2)+2]$ or $(3x+8)(3x+4)$
80. .
81. $(6a-7)(6a+7)$
82. .
83. $(a+b)(a^2 -ab + b^2)$ --> $(3x+y)(9x^2-3xy+y^2)$
84. .
85. $(a-b)(a^2 +ab + b^2)$ --> $(2s-5t)(4s^2-10st+25t^2)$
86. .
87. $(x+6)^2$
88. .
89. $x^2(x+4)+(x+4)$ = $(x^2+1)(x+4)$
90. .
91. $x^2(5x+1)+(5x+1)$ = $(2x^2+1)(5x+1)$
92. .
93. $x^2(x+1)+(x+1)$ = $(x^2+1)(x+1)$
94. .
95. $x^{2/3}(1 + 3x)$
96. .
97. $x^{-1/2}(x^{-1}-1+x)$
98. .
99. $(2x^2+1)^{-1/2}[(2x^2+1)+2]$ = $(2x^2+1)^{-1/2}(2x^2+3)$
100. .
101. $2x(6x^2+1)$
102. .
103. $(x-4)(x+2)$
104. .
105. $(2x+3)(x+1)$
106. .
107. $(3x-15)(3x+3)$
108. .
109. $(7-2y)(7+2y)$
110. .
111. $(t-3)^2$
112. .
113. $(y-5z)^2$
114. .
115. $[(a+b)-(a-b)][(a+b)+(a-b)]$
116. .
117. $(x^2-9)(x^2-1)$
118. .
119. $(a-b)(a^2+ab+b^2)$ --> $(2x-5)(4x^2-10x+25)$
120. .
121. $x(x^2+2x+1)$ = $x(x+1)^2$
122. .
123. $x^2y^3(x^2-y^2)$ = $x^2y^3(x-y)(x+y)$
124. .
125. $x^2(3x-1)-4(3x-1)$ = $(x^2-4)(3x-1)$
126. .
127. $x^{-1/2}(x^{-1}+2+x)$
128. .
129. $(x-1)(x+2)[(x+2)-(x-1)]$ = $3(x-1)(x+2)$
130. .
131. $[(a^2+1)-5][(a^2+1)-2]$
132. .
133. $(x-1)^3[(x^2+3)^2-(4x+1)^2]$ <-- too cumbersome.
134. .
135. $2(x^2+4)^4(x-2)^3[5x(x-2)+2(x^2+4)]$
136. .
137. $a^{-1/3}-\frac{2}{3}x^2a^{-4/3}$ = $a^{-1/3}\left( 1-\frac{2}{3}x^2a^{-1} \right)$ --> $(x^2+3)^{-1/3}\left[ 1-\frac{2}{3}x^2(x^2+3)^{-1} \right]$
138. .

## Skills Plus

139. (a) $\frac{1}{2}[a^2+2ab+b^2-a^2-b^2]$ = $\frac{1}{2}(2ab)$ = $ab$ (b) $(a^4+2a^2b^2+b^4)-(a^4-2a^2b^2+b^4)$ = $4a^2b^2$
140. .
141. Skip
142. .

## Applications

143. For cylinder, the volume is $V = \pi r^2h$. For culvert, the volume is $V = \pi R^2h-\pi r^2h$. This makes sense, since culvert is basically a cylinder minus a smaller cylinder. Factoring the volume formula for culvert, we get $V = \pi h(R^2-r^2)$. Another formula for culvert is $V = 2\pi \cdot \text{average radius} \cdot \text{height} \cdot \text{thickness}$, or $V = 2\pi\left( \frac{R+r}{2} \right)h(R-r)$. This formula is equivalent to the previous formula because it simplifies to $V = \pi h(R+r)(R-r)$, which is what you get when you factor $V = \pi h(R^2-r^2)$. It makes sense geometrically as well :
     ![[Pasted image 20250915134310.png]]


## Incorrect

- 7) $(A + B)^2$, $(x + 5)^2$
- 19) $5x^3+4x^2-3x-x^2-7x-2$ = $5x^3+3x^2-10x-2$
- 55) $x-2x^{1/2}y^{1/2}+y$
- 97) $x^{-3/2}(1-x+x^2)$
- 99)
- 107)
- 115)
- 117)
- 125)
- 127)
- 131)
- 133)
- 135)
- 137)