# 1.5 Exercises

## Concepts

1. (a) yes (b) yes (c) no, squaring introduces extraneous solutions.
2. (a) square root on both sides (b) apply $-5$ on both sides (c) apply $-2$ on both sides
3. (a) $(x-8)(x+2)=0$ (b) $x^2-6x+9=16+9$ = $(x-3)^2=25$ = $x-3 = \pm 5$ = $x = \pm 5 +3$ (c) $x=\frac{6 \pm \sqrt{ 36-4(-16) }}{2}$ = $x=3 \pm 5$
4. (a) $0$ (b) $0, 4$ (c) factor
5. (a) $\sqrt{ 2x } = -x$ (b) $2x = x^2$ (c) $0,2$ (d) $0$
6. quadratic type, $W = x+1$, $W^2-5W+6=0$
7. $x(x+2)$, $3(x+2)+5x=2x(x+2)$ = $3x+6+5x=2x^2+4$ = $-2x^2+8x+2=0$ = $x^2-4x-1=0$
8. square, $(2x+1)^2=x+1$

## Skills

9. (a) no (b) yes
10. .
11. (a) yes (b) no
12. .
13. linear, $x=-1$
14. .
15. linear, $x=18$
16. .
17. equivalent, $x=\frac{3}{5}$
18. .
19. equivalent, $-\frac{4x}{3}=9$ = $x=-\frac{27}{4}$
20. .
21. equivalent, $2-2x=3+6x+5$ = $-8x=6$ = $x=-\frac{3}{4}$
22. .
23. equivalent, $x=30$
24. .
25. equivalent, $5(2x-1)=4(x+2)$ = $10x-5=4x+8$ = $x=\frac{13}{6}$
26. .
27. equivalent, $x=-\frac{1}{3}$
28. .
29. $m=\frac{2E}{v^2}$
30. .
31. $w=\frac{P}{2}-l$
32. .
33. $x=\frac{2d-b}{a-2c}$
34. .
35. $a^2x-(a+1)x=-(a-1)$ = $x(a^2-a-1)=-(a-1)$ = $x=-\frac{a-1}{a^2-a-1}$
36. .
37. $r^2=\frac{3V}{\pi h}$ = $r = \pm \sqrt{ \frac{3V}{\pi h} }$
38. .
39. $b= \pm \sqrt{ c^2-a^2 }$
40. .
41. $x^2+x-12=0$ = $(x+4)(x-3)=0 \implies x=-4 \text{ or } x=3$
42. .
43. $(x+15)(x-2)=0 \implies x=-15 \text{ or } x=2$
44. .
45. $(2x-5)(2x+3)=0 \implies x=\frac{5}{2} \text{ or } x= -\frac{3}{2}$
46. .
47. $x=\pm 2$
48. .
49. $2x-5= \pm 9 \implies x=7 \text{ or } x=-2$
50. .
51. $(x+5)^2=2$ = $x+5= \pm \sqrt{ 2 } \implies x=\pm \sqrt{ 2 }-5$
52. .
53. $x^2+10x=-2$ = $x^2+10x+25=-2$ = $(x+5)^2=-2$ = $x+5= \pm \sqrt{ -2 } \implies x=\pm \sqrt{ -2 }-5$ or there is no real solution
54. .
55. $x^2-6x=11$ = $x^2-6x+9=11$ = $(x-3)^2=11$ = $x-3= \pm \sqrt{ 11 } \implies x=\pm \sqrt{ 11 }+3$
56. .
57. $x^2+2x=\frac{1}{5}$ = $(x+1)^2=\frac{1}{5}$ = $x+1 = \pm \sqrt{ \frac{1}{5} } \implies x=\pm \sqrt{ \frac{1}{5} }-1$
58. .
59. $x^2-\frac{1}{4}x+\frac{1}{64}=0$ = $\left( x-\frac{1}{8} \right)^2=0 \implies x=\frac{1}{8}$
60. .
61. $\frac{2 \pm \sqrt{ 4-4(-15) }}{2}$ = $x= 1 \pm 4$
62. .
63. $\frac{-1 \pm \sqrt{ 1-4(2)(-3) }}{4}$ = $x= -\frac{1}{4} \pm \frac{5}{4}$
64. .
65. $\frac{-6 \pm \sqrt{ 36-4(3)(-5) }}{6}$ = $x= -1 \pm \frac{2\sqrt{ 6 }}{3}$
66. .
67. $\frac{-12 \pm \sqrt{ 144-4(9)(4) }}{18}$ = $x=-\frac{2}{3}$
68. .
69. $4x^2+16x-9=0$ = $\frac{-16 \pm \sqrt{ 256-4(4)(-9) }}{8}$ = $x = -2 \pm \frac{5}{2}$
70. .
71. $7x^2-2x+4=0$ = $\frac{4 \pm \sqrt{ 2-4(7)(4) }}{14}$ = $\frac{2}{7} \pm \frac{\sqrt{ -110 }}{14}$. There is no real solution.
72. .
73. two real solutions
74. .
75. one real solution
76. .
77. no solution
78. .
79. $x^2=50(x+100)$ = $x^2 = 50x + 5000$ = $x^2-50x-5000=0 \implies x=100 \text{ or } x=-50$
80. .
81. $(y+1)(y+2)=2(y^2+1)$ = $y^2+3y+2=2y^2+2$ = $y^2-3y=0$ = $y(y-3)=0 \implies y=0 \text{ or } y=3$
82. .
83. $(x+2)+(x-1)=\frac{5(x-1)(x+2)}{4}$ = $2x+1=\frac{5(x^2+x-2)}{4}$ = $8x+4=5x^2+5x-10$ = $5x^2-3x-14=0$ = $(5x+7)(x-2) = 0 \implies x=-\frac{7}{5} \text{ or } x= 2$
84. .
85. $x=7$
86. .
87. $2x-1 = 3x-5$ = $x=4$
88. .
89. $2x+1=(x-1)^2$ = $2x+1 = x^2-2x+1$ = $x^2-4x=0$ = $x(x-4)=0 \implies x=0 \text{ or } x=4$
90. .
91. $W^2-13W+40=0$ = $(W-8)(W-5)=0$ = $x^2=8, x^2=5$ = $x=\pm 2\sqrt{ 2 }, x=\pm \sqrt{ 5 }$
92. .
93. $W^2-5W+4=0$ = $(W-4)(W-1)=0$ = $(x+2)^2=4, (x+2)^2=1$ = $x(x+4)=0, (x+3)(x+1)=0 \implies x \in \{ 0,-4,-3,-1 \}$
94. .
95. $W^2-5W+6=0$ = $(W-3)(W-2)=0$ = $(x^{2/3}-3)(x^{2/3}-2)=0 \implies x=\pm 3\sqrt{ 3 } \text{ or } x=\pm 2\sqrt{ 2 }$
96. .
97. $x^{1/2}+3x^{-1/2}-10x^{-3/2}=0$ = $x^{-3/2}(x^2+3x-10)=0 \implies x \in \{ 0,-5,2 \}$, but $x=-5$ might not be a solution...
98. .
99. $3x+5=1, 3x+5=-1$ = $3x=-4, 3x=-6$ = $x=-\frac{4}{3}, -2$
100. .
101. $x-4=0.01, x-4=-0.01$ = $x=4.01,3.99$
102. .
103. $x=-2$
104. .
105. $a=\frac{4}{3},-1$
106. .
107. $y=\frac{21}{11}$
108. .
109. $x=\frac{-3+3\sqrt{ 5 }}{2}$
110. .
111. $x=256$
112. .
113. $x=13, -\frac{19}{3}$
114. .
115. $z=6,4$
116. .
117. $3x^2-1=11, -11$ = $3x^2=12,-10$ = $x^2=4,-\frac{10}{3}$ = $x=-2,2$
118. .

## Skills Plus

119. $x=-\frac{1}{2}$
120. .
121. $x=5$
122. .
123. $x=-3$
124. .
125. $(x^2-4a)(x^2-a)=0$ = $x^2=4a, a$ = $x= \pm 2\sqrt{ a }, \pm \sqrt{ a }$ (I guess as long as $a=1$)
126. .
127. $x=\frac{a^2-36}{12}$ = $x=\frac{a^2}{12}-3$
128. .

## Applications

129. $t= \pm 3\sqrt{ 2 }$
130. .
131. (a) $t=1, \frac{3}{2}$ (b) it doesn't? (c) $25$ ft (d) $t=\frac{5}{4}$ (e) $t=\frac{5}{2}$
132. .
133. (a) $S=0.00055$, $12.02445$ (b) $234.375 \text{ kg/m\(^3\)}$
134. .


### 135. The Bernoulli Equation

If a fluid with density $p$ (kg/m³) is pumped with velocity $v$ (m/s) through a given pipe, then the pressure $P$ (Pa) in the pipe satisfies Bernoulli's equation

$$
\frac{1}{2}pv^2 + pgh + P = C
$$

where $h$ is the height (m) above some fixed reference point, $g$ is acceleration due to gravity ($9.81$ m/s²), and $C$ is a constant specific to the given pipe.

![[Pasted image 20250926100107.png]]

Suppose water ($p = 1000$ kg/m³) is flowing through a pipe at height $1$ m, with velocity $2$ m/s and pressure $20,000$ Pa.

---
**(a)** Find the constant $C$ for the pipe.

Given :
- $p = 1000$
- $h = 1$
- $v = 2$
- $g = 9.81$
- $P = 20000$

Equation : 

Answer : 

---
**(b)** Solve for the variable $P$ in Bernoulli's equation. If the height increases to $5$ m, what is the new pressure? If the height returns to $1$ m and the velocity increases to $4$ m/s, what is the new pressure?

$$
\begin{align}
  P &= C-\frac{1}{2}pv^2-pgh
\end{align}
$$


---


### 137. Gravity

If an imaginary line segment is drawn between the centers of the Earth and the Moon, then the net gravitational force $F$ acting on an object situated on this line segment is

$$
F = -\frac{K}{x^2} + \frac{0.012K}{(239-x)^2}, (0 < x < 239)
$$

where $K>0$ is a constant and $x$ is the distance of the object from the center of the Earth, measured in thousands of miles.

![[Pasted image 20250926103628.png]]

How far from the center of the Earth is the "dead spot" where no net gravitational force acts upon the object? (Round to the nearest thousand miles)

---

$$
\begin{align}
  0 &= -\frac{K}{x^2}+\frac{0.012K}{(239-x)^2} \\
  0 &= -\frac{1}{x^2} + \frac{0.012}{(239-x)^2} \\
  0 &= -(239-x)^2+0.012x^2 \\
  0 &= x^2+478x-57121
\end{align}
$$





---


## Incorrect

