# 1.6 Exercises

## Concepts

1. $-1$
2. $3$, $4$
3. (a) $3-4i$ (b) $25$
4. $3-4i$
5. Yes
6. Yes

## Skills

7. $3$, $-8$
8. .
9. $-\frac{2}{3}$, $-5/3$
10. .
11. $3$, $0$
12. .
13. $0$, $-\frac{2}{3}$
14. .
15. $\sqrt{ 3 }$, $2$
16. .
17. $3+7i$
18. .
19. $1-10i$
20. .
21. $3+5i$
22. .
23. $2-2i$
24. .
25. $-19+4i$
26. .
27. $-4+8i$
28. .
29. $6+15i-8i+20$ = $26+7i$
30. .
31. $12-18i+10i+15$ = $27-8i$
32. .
33. $13$
34. .
35. $9-12i-4$ = $5-12i$
36. .
37. $\frac{1}{i}$ = $-\frac{i}{1}$ = $-i$
38. .
39. $\frac{1-3i}{1+2i} \cdot \frac{1-2i}{1-2i}$ = $\frac{1-5i-6}{5}$ = $\frac{-5-5i}{5}$ = $-1-i$
40. .
41. $\frac{10i}{1-2i} \cdot \frac{1+2i}{1+2i}$ = $\frac{10i-20}{5}$ = $-4+2i$
42. .
43. $\frac{4+6i}{3i} \cdot \frac{3i}{3i}$ = $\frac{12i-18}{-9}$ = $2-\frac{4}{3}i$
44. .
45. $\frac{1-i}{2}-\frac{1+i}{2}$ = $-i$
46. .
47. $-i$
48. .
49. $243i$
50. .
51. $1$
52. .
53. $5i$
54. .
55. $-6$
56. .
57. $6-2i\sqrt{ 3 }+3i+\sqrt{ 3 }$ = $(6+\sqrt{ 3 })+(3i-2i\sqrt{ 3 })$
58. .
59. $\frac{2+i\sqrt{ 8 }}{1+i\sqrt{ 2 }} \cdot \frac{1-i\sqrt{ 2 }}{1-i\sqrt{ 2 }}$ = $\frac{2-2i\sqrt{ 2 }+i\sqrt{ 8 }+4}{1+2}$ = $\frac{6}{3}$ = $2$
60. .
61. $x=\pm 5i$
62. .
63. $x = \frac{6 \pm \sqrt{ 36-4(13) }}{2}$ = $x = \frac{6 \pm \sqrt{ -16 }}{2}$ = $x = 3 \pm 2i$
64. .
65. $x = \frac{2 \pm \sqrt{ 4-4(2)(5) }}{4}$ = $x = \frac{2 \pm \sqrt{ -36 }}{4}$ = $x = \frac{2 \pm 6i}{4}$ = $x = \frac{1}{2} \pm \frac{3}{2}i$
66. .
67. $x = \frac{-1 \pm \sqrt{ -3 }}{2}$ = $x = -\frac{1}{2} \pm \frac{\sqrt{ 3 }}{2}i$
68. .
69. $x = \frac{4 \pm \sqrt{ 16 - 4(9)(4) }}{18}$ = $x = \frac{4 \pm \sqrt{ -128 }}{18}$ = $x = \frac{2}{9} \pm \frac{4i\sqrt{ 2 }}{9}$
70. .
71. $x = \frac{-12 \pm \sqrt{ 144 - 4(6)(7) }}{12}$ = $x = -1 \pm \frac{i\sqrt{ 6 }}{6}$
72. .

## Skills Plus

73. $(3+4i)+(5-2i)$ = $8+2i$
74. .
75. $(3-4i)(3+4i)$ = $9+16$ = $25$
76. .
77. $(a-bi)+(c-di)=(a+c)-(bi+di)$, $(a+bi)+(c+di)=(a+c)+(bi+di)$, conjugate is $(a+c)-(bi+di)$. Ergo, $\overline{z}+\overline{w}=\overline{z+w}$
78. .
79. $(a-bi)^2 = a^2-2abi-b^2 = (a^2-b^2)-2abi$, $(a+bi)^2=a^2+2abi-b^2 = (a^2-b^2)+2abi$, conjugate is $(a^2-b^2)-2abi$. Thus, $(\overline{z})^2 = \overline{z^2}$
80. .
81. $(a+bi)+(a-bi)=2a$, it is a real number
82. .
83. $(a+bi)(a-bi) = a^2+b^2$, it is a real number


## Incorrect

None! (not really but small mistakes were fixed)