# 1.4 Exercises

## Concepts

1. Both (a) and (c) are rational expressions. (b) is not a rational expression because there is a radical in the numerator.
2. Numerator, Denominator, $\frac{x+1}{x+3}$
3. Numerator, Denominator, $\frac{2x}{(x+1)(x+3)}$
4.  (a) $3$ (b) $x(x+1)^2$ (c) $\frac{(x+1)^2}{x(x+1)^2} - \frac{2x(x+1)}{x(x+1)^2} - \frac{x^2}{x(x+1)^2}$ = $\frac{-2x^2+1}{x(x+1)^2}$
5. (a) yes (b) no
6. (a) yes (b) no


## Skills

7. $\{ x \in \mathbb{R} \}$
8. .
9. $\{ x \mid x \neq 3 \}$
10. .
11. $\{ x \mid x \geq -3 \}$
12. .
13. $\{ x \mid x \neq 2 \text{ and } x \neq -1 \}$
14. .
15. $\{ x \mid x \geq 2 \}$
16. .
17. $\frac{x+5}{2}$
18. .
19. $\frac{1}{x+2}$
20. .
21. $\frac{(x-8)(x+1)}{(x-8)(x-2)}$ = $\frac{x+1}{x-2}$
22. .
23. $\frac{y(y+1)}{(y-1)(y+1)}$ = $\frac{y}{y-1}$
24. .
25. $\frac{x(2x^2-x-6)}{2x^2-7x+6}$ = $\frac{x(2x+3)(x-2)}{(2x-3)(x-2)}$ = $\frac{x(2x+3)}{2x-3}$
26. .
27. $\frac{4x(x+2)}{16x(x^2-4)}$ = $\frac{x+2}{4(x-2)(x+2)}$ = $\frac{1}{4(x-2)}$
28. .
29. $\frac{(x+5)(x-3)}{(x-5)(x+5)} \cdot \frac{x-5}{x+2}$ = $\frac{x-3}{x+2}$
30. .
31. $\frac{2t+3}{t^2+9} \cdot \frac{2t-3}{4t^2-9}$ = $\frac{4t^2-9}{(t^2+9)(4t^2-9)}$ = $\frac{1}{t^2+9}$
32. .
33. $\frac{(x-4)(x+2)}{(x+6)(x+2)} \cdot \frac{(x+6)(x-4)}{x(x-4)(x+4)}$ = $\frac{x-4}{x+6} \cdot \frac{x+6}{x(x+4)}$ = $\frac{x-4}{x(x+4)}$
34. .
35. $\frac{x+3}{(2x-3)(2x+3)} \cdot \frac{(2x-3)(x+5)}{(x+4)(x+3)}$ = $\frac{x+5}{(2x+3)(x+4)}$
36. .
37. $\frac{x^3}{x+1} \cdot \frac{(x+1)(x+1)}{x}$ = $x^2(x+1)$
38. .
39. $\frac{x}{y} \cdot \frac{1}{z}$ = $\frac{x}{yz}$
40. .
41. $\frac{x+4}{x+3}$
42. .
43. $\frac{x-3}{(x+5)(x-3)} + \frac{2(x+5)}{(x+5)(x-3)}$ = $\frac{3x+7}{(x+5)(x-3)}$
44. .
45. $\frac{3(x+2)}{(x+2)(x+1)} - \frac{x+1}{(x+2)(x+1)}$ = $\frac{2x+5}{(x+2)(x+1)}$
46. .
47. $\frac{5(2x-3)}{(2x-3)^2} - \frac{3}{(2x-3)^2}$ = $\frac{10x-18}{(2x-3)^2}$ = $\frac{2(5x-9)}{(2x-3)^2}$
48. .
49. $\frac{u^2+3u+1}{u+1}$
50. .
51. $\frac{x^2+x}{x^2(x^2+x)} + \frac{x^2}{x^2(x^2+x)}$ = $\frac{2x^2+x}{x^2(x^2+x)}$ = $\frac{x(2x+1)}{x^3(x+1)}$ = $\frac{2x+1}{x^2(x+1)}$
52. .
53. $\frac{2(x+4)}{(x+3)(x+4)} - \frac{1}{(x+3)(x+4)}$ = $\frac{2x+7}{(x+3)(x+4)}$
54. .
55. $\frac{x-3}{(x+3)(x-3)} + \frac{1}{(x-3)(x+3)}$ = $\frac{x-2}{(x+3)(x-3)}$
56. .
57. $\frac{2(x-1)}{x(x-1)} + \frac{3x}{x(x-1)} - \frac{4}{x(x-1)}$ = $\frac{5x-6}{x(x-1)}$
58. .
59. $\frac{x(x+1)}{x^3(x+1)^2} + \frac{x}{x^3(x+1)^2} + \frac{1}{x^3(x+1)^2}$ = $\frac{(x+1)(x+1)}{x^3(x+1)^2}$ = $\frac{1}{x^3}$
60. .
61. $\frac{x+1}{x} \cdot \frac{x}{-2x+1}$ = $\frac{x+1}{-2x+1}$
62. .
63. $\frac{x+3}{x+2} \cdot \frac{x+2}{x+1}$ = $\frac{x+3}{x+1}$
64. .
65. $(\frac{x+3}{(x-1)(x+3)} + \frac{x-1}{(x-1)(x+3)}) \cdot \frac{1}{x+1}$ = $\frac{2(x+1)}{(x-1)(x+3)} \cdot \frac{1}{x+1}$ = $\frac{2}{(x-1)(x+3)}$
66. .
67. $\frac{xy-x}{y} \cdot \frac{xy-y}{x}$ = $\frac{x(y-1)}{y} \cdot \frac{y(x-1)}{x}$ = $(y-1)(x-1)$
68. .
69. $\frac{x^2-y^2}{xy} \cdot -\frac{x^2y^2}{x^2-y^2}$ = $-xy$
70. .
71. $(x^{-1}-y^{-1})(x^{-1}+y^{-1}) \cdot \frac{1}{x^{-1}+y^{-1}}$ = $x^{-1}-y^{-1}$ or $\frac{1}{x} - \frac{1}{y}$ or $\frac{y-x}{xy}$
72. .
73. $1 - \frac{x}{x-1}$ = $\frac{x-1}{x-1}-\frac{x}{x-1}$ = $-\frac{1}{x-1}$ or $\frac{1}{1-x}$
74. .
75. $\frac{\frac{1}{1+x+h}-\frac{1}{1+x}}{h}$ = $-\frac{h}{(1+x)(1+x+h)} \cdot \frac{1}{h}$ = $-\frac{1}{(1+x)(1+x+h)}$
76. .
77. $-\frac{h(h+2x)}{x^2(x+h)^2} \cdot \frac{1}{h}$ = $-\frac{h+2x}{x^2(x+h)^2}$
78. .
79. $\sqrt{ \frac{1}{(1-x)(1+x)} }$ = $\frac{1}{\sqrt{ (1-x)(1+x) }}$ = $\frac{\sqrt{ (1-x)(1+x) }}{(1-x)(1+x)}$
80. .
81. $\frac{(x-3)(-x+19)}{(x+5)^4}$
82. .
83. $\frac{(x+1)^{-1/2}(x+2)}{x+1}$ = $\frac{x+2}{(x+1)^{3/2}}$
84. .
85. $\frac{(1+x)^{-2/3}(2x+3)}{(1+x)^{2/3}}$ = $\frac{2x+3}{(1+x)^{4/3}}$
86. .
87. $\frac{3-\sqrt{ 10 }}{9-10}$ = $-3+\sqrt{ 10 }$
88. .
89. $\frac{2(\sqrt{ 5 }+\sqrt{ 3 })}{5-3}$ = $\sqrt{ 5 }+\sqrt{ 3 }$
90. .
91. $\frac{y(\sqrt{ 3 } - \sqrt{ y })}{3-y}$
92. .
93. $-\frac{1}{5(2+\sqrt{ 5 })}$
94. .
95. $\frac{r-2}{5(\sqrt{ r } - \sqrt{ 2 })}$
96. .
97. $\frac{1}{\sqrt{ x^2+1 }+x}$
98. .

## Applications

99. (a) $\frac{R_{1}R_{2}}{R_{2}+R_{1}}$ (b) $\frac{(10)(20)}{20+10}$ = $\frac{200}{30}$ = $\frac{20}{3}$


## Incorrect

- 33) $\frac{x(x-4)(x+2)}{(x+6)(x+2)} \cdot \frac{(x+6)(x-4)}{x(x-4)(x+4)}$ = $\frac{x(x-4)}{(x+6)} \cdot \frac{(x+6)}{x(x+4)}$ = $\frac{x-4}{x+4}$
- 67) $\frac{xy-x}{y} \cdot \frac{x}{xy-y}$ = $\frac{x^2(y-1)}{y^2(x-1)}$

